Working on the separate compilation for symbol table gen

x86/RelocProgram.v
@@ -220,20 +220,20 @@ Definition sec_rel_code_id := 6%N.
 Definition sec_shstrtbl_id := 7%N.
 
 (** Ultility function s*)
-Definition add_symb_to_tree (s:symbentry) (t: PTree.t symbentry) :=
+Definition add_symb_to_tree (t: PTree.t symbentry) (s:symbentry) :=
   match symbentry_id s with
   | None => t
   | Some id => PTree.set id s t
   end.
 
 Definition symbtable_to_tree (t:symbtable) : PTree.t symbentry :=
-  fold_right add_symb_to_tree (PTree.empty symbentry) t.
+  fold_left add_symb_to_tree t (PTree.empty symbentry).
 
-Definition acc_symb_ids (s:symbentry) (ids: list ident) :=
+Definition acc_symb_ids (ids: list ident) (s:symbentry) :=
   match symbentry_id s with
   | None => ids
   | Some id => id :: ids
   end.
 
 Definition get_symbentry_ids (t:symbtable) : list ident :=
-  fold_right acc_symb_ids nil t.
+  fold_left acc_symb_ids t nil.
